@prefix : <https://w3id.org/riskman/ontology/security#> .
@prefix dc: <http://purl.org/dc/elements/1.1/> .
@prefix dcterms: <http://purl.org/dc/terms/> .
@prefix owl: <http://www.w3.org/2002/07/owl#> .
@prefix rdf: <http://www.w3.org/1999/02/22-rdf-syntax-ns#> .
@prefix xml: <http://www.w3.org/XML/1998/namespace> .
@prefix xsd: <http://www.w3.org/2001/XMLSchema#> .
@prefix rdfs: <http://www.w3.org/2000/01/rdf-schema#> .
@prefix schema: <https://schema.org/> .
@prefix vann: <http://purl.org/vocab/vann/> . 
@prefix riskman: <https://w3id.org/riskman/ontology#> .
@prefix rlevel: <https://w3id.org/riskman/ontology#> .
@prefix rsecurity: <https://w3id.org/riskman/ontology/security#> .
@prefix ontogs: <https://www.npmjs.com/package/ontoglimpse#> .
@base <https://w3id.org/riskman/ontology/security#> .

<https://w3id.org/riskman/ontology> 
                                      rdf:type owl:Ontology ;
                                      dcterms:description "An extension of the Riskman ontology that also takes in account security aspects of medical devices." ;
                                      dcterms:license <http://creativecommons.org/licenses/by/4.0/> ;
                                      dcterms:title "Experimental section" ; 
                                      dcterms:created "2024-08-20"^^xsd:date ;
                                      rdfs:label "Extension of the Riskman Ontology for Security" ;
                                      schema:dateModified "2024-11-13"^^xsd:date ;
                                      vann:preferredNamespacePrefix "rsecurity"  ;
                                      vann:preferredNamespaceURI "https://w3id.org/riskman/ontology/security#" ;
                                      ontogs:customSwitch1 "true" .


#################################################################
#    Object Properties
#################################################################


###  https://w3id.org/riskman/ontology/security#hasJustification
:hasJustification rdf:type owl:ObjectProperty ;
           rdfs:domain riskman:Risk ;
           rdfs:range :Justification ;
           rdfs:label "has justification" .




#################################################################
#    Classes
#################################################################


###  https://w3id.org/riskman/ontology/security#SecurityHazard
:SecurityHazard rdf:type owl:Class ;
                rdfs:subClassOf riskman:Hazard ;
                rdfs:comment "A security-related hazard: one of availability, confidentiality, or integrity" ;
                rdfs:label "Security hazard" .




###  https://w3id.org/riskman/ontology/security#AnalyzedSecurityRisk
:AnalyzedSecurityRisk rdf:type owl:Class ;
                      rdfs:subClassOf riskman:AnalyzedRisk ;
                      rdfs:comment "A security-related analyzed risk: an analyzed risk having a domain-specific hazard with a security hazard" ;
                      rdfs:label "Analyzed security risk" .


[ owl:intersectionOf ( riskman:AnalyzedRisk
                       [ rdf:type owl:Restriction ;
                         owl:onProperty riskman:hasDomainSpecificHazard ;
                         owl:someValuesFrom [ rdf:type owl:Restriction ;
                                              owl:onProperty riskman:hasHazard ;
                                              owl:someValuesFrom :SecurityHazard
                                            ]
                       ]                      
                     ) ;
  rdf:type owl:Class ;
  rdfs:subClassOf :AnalyzedSecurityRisk
] .




###  https://w3id.org/riskman/ontology/security#ControlledSecurityRisk
:ControlledSecurityRisk rdf:type owl:Class ;
                        rdfs:subClassOf riskman:ControlledRisk ;
                        rdfs:comment "A security-related controlled risk: a controlled risk having an analyzed security risk" ;
                        rdfs:label "Controlled security risk" .


[ owl:intersectionOf ( riskman:ControlledRisk
                       [ rdf:type owl:Restriction ;
                         owl:onProperty riskman:hasAnalyzedRisk ;
                         owl:someValuesFrom :AnalyzedSecurityRisk
                       ]
                     ) ;
  rdf:type owl:Class ;
  rdfs:subClassOf :ControlledSecurityRisk
] .




###  https://w3id.org/riskman/ontology/security#Justification
:Justification rdf:type owl:Class;
               rdfs:comment "Further justification associated to a risk (mainly intended to justify risk levels)";
               rdfs:label "Justification" .




###  https://w3id.org/riskman/ontology/security#RiskLevelNeedingJustification
:RiskLevelNeedingJustification rdf:type owl:Class ;
                rdfs:subClassOf riskman:RiskLevel ;
                rdfs:comment "A risk level that needs further justification" ;
                rdfs:label "Risk level needing justification" .






#################################################################
#    Individuals
#################################################################

###  https://w3id.org/riskman/ontology/security#Availability
:Availability rdf:type owl:NamedIndividual , :SecurityHazard ;
                             rdfs:label "Availability" .



###  https://w3id.org/riskman/ontology/security#Confidentiality
:Confidentiality rdf:type owl:NamedIndividual , :SecurityHazard ;
                             rdfs:label "Confidentiality" .


###  https://w3id.org/riskman/ontology/security#Integrity
:Integrity rdf:type owl:NamedIndividual , :SecurityHazard ;
                          rdfs:label "Integrity" .




